compiler1/semantics/conPropsScript.sml
@@ -17,4 +17,31 @@ val build_rec_env_merge = Q.store_thm ("build_rec_env_merge",
     MAP (λ(fn,n,e). (fn, Recclosure env funs fn)) funs ++ env'`,
   rw [build_rec_env_def, build_rec_env_help_lem]);
 
+val pat_bindings_accum = Q.store_thm ("pat_bindings_accum",
+  `(!p acc. pat_bindings p acc = pat_bindings p [] ++ acc) ∧
+   (!ps acc. pats_bindings ps acc = pats_bindings ps [] ++ acc)`,
+  Induct >>
+  rw []
+  >- rw [pat_bindings_def]
+  >- rw [pat_bindings_def]
+  >- metis_tac [APPEND_ASSOC, pat_bindings_def]
+  >- metis_tac [APPEND_ASSOC, pat_bindings_def]
+  >- rw [pat_bindings_def]
+  >- metis_tac [APPEND_ASSOC, pat_bindings_def]);
+
+val Boolv_11 = store_thm("Boolv_11[simp]",
+  ``Boolv b1 = Boolv b2 ⇔ (b1 = b2)``, EVAL_TAC >> rw[])
+
+val evaluate_list_length = Q.store_thm ("evaluate_list_length",
+  `!b env s gtagenv es s' vs.
+    conSem$evaluate_list b env s es (s', Rval vs)
+    ⇒
+    LENGTH es = LENGTH vs`,
+  induct_on `es` >>
+  rw [] >>
+  Cases_on`vs`>>
+  pop_assum (mp_tac o SIMP_RULE (srw_ss()) [Once conSemTheory.evaluate_cases]) >>
+  rw [] >>
+  metis_tac []);
+
 val _ = export_theory()
